example/slippage/formal_verification/lakefile.lean
@@ -6,6 +6,9 @@ package slippageProofs
 require qedgenSupport from
   "./lean_support"
 
+lean_lib SlippageProg where
+  roots := #[`SlippageProg]
+
 @[default_target]
 lean_lib SlippageProofs where
   roots := #[`SlippageProofs]
