example/transfer/formal_verification/lakefile.lean
@@ -6,6 +6,9 @@ package transferProofs
 require qedgenSupport from
   "./lean_support"
 
+lean_lib TransferProg where
+  roots := #[`TransferProg]
+
 @[default_target]
 lean_lib TransferProofs where
   roots := #[`TransferProofs]
